iris/UkShEcho.v
@@ -940,14 +940,16 @@ Section UkShEcho.
   (* must exec on the pin too, so [UserCwd.ucwd_any] in                    *)
   (* [UkSh.ush_pstate] becomes [ucwd (ukn_cwd N) ROOTINO] here.            *)
   (* =================================================================== *)
-  Definition ush_pstate_at (N : uk_names Σ) (gp : gname) (l : list fdstate)
-      (c : Z) : iProp Σ :=
+  (* [T] IS A PARAMETER (lane IO-LEAF, M5(3)): the fourth conjunct is the
+     cursor AT A LINE BOUNDARY now, whose other arm is the taint. *)
+  Definition ush_pstate_at (N : uk_names Σ) (gp : gname) (T : iProp Σ)
+      (l : list fdstate) (c : Z) : iProp Σ :=
     (UkSh.ush_std N l ∗ UserCwd.ucwd (ukn_cwd N) c
-     ∗ UserChildren.uch_any (ukn_ch N) ∗ UkSh.ush_pos N gp)%I.
+     ∗ UserChildren.uch_any (ukn_ch N) ∗ UkSh.ush_posb N gp T)%I.
 
-  Lemma ush_pstate_of_at (N : uk_names Σ) (gp : gname) (l : list fdstate)
-      (c : Z) :
-    ush_pstate_at N gp l c -∗ UkSh.ush_pstate N gp l.
+  Lemma ush_pstate_of_at (N : uk_names Σ) (gp : gname) (T : iProp Σ)
+      (l : list fdstate) (c : Z) :
+    ush_pstate_at N gp T l c -∗ UkSh.ush_pstate N gp T l.
   Proof.
     rewrite /ush_pstate_at /UkSh.ush_pstate.
     iIntros "(Hstd & Hcwd & Hch & Hpos)". iFrame "Hstd Hch Hpos".
@@ -959,8 +961,8 @@ Section UkShEcho.
      fork arm threads through both processes' entry and back out of the
      parent's ([UkShFork.wp_kshf_fork]). *)
   Definition ush_echo_round_carry (N : uk_names Σ) (gp : gname)
-      (l : list fdstate) (sz : Z) (f : nat -> bv 8) : iProp Σ :=
-    (ush_pstate_at N gp l FsImg.ROOTINO
+      (T : iProp Σ) (l : list fdstate) (sz : Z) (f : nat -> bv 8) : iProp Σ :=
+    (ush_pstate_at N gp T l FsImg.ROOTINO
      ∗ UkShLoop.ushl_dat (ukn_d N) ∗ usz (ukn_s N) sz
      ∗ ubytes (ukn_d N) UkSh.sh_buf UkSh.sh_nbuf f)%I.
 
